Removed remaining sorry in ViperBoogieRelUtil, which was achieved by adjusting the state relation.
There is now an option that controls whether the state consistency should be enforced, which allows one to derive the state relation w.r.t. a consistent Viper state via intermediate "helper" Viper states that may not be consistent (for example, updating the heap and mask in separate steps).
Another minor change is that heap_var_rel and mask_var_rel directly take the field translation as a parameter instead of the entire translation record.

ViperBoogieBasicRel.thy
@@ -29,6 +29,12 @@ datatype boogie_const =
 definition total_context_trivial :: "program \<Rightarrow> 'a total_context"
   where "total_context_trivial Pr \<equiv> \<lparr> program_total = Pr, fun_interp_total=f_None, absval_interp_total=(\<lambda>_.''dummy'')  \<rparr>"
 
+text \<open>The following records tracks options controlling whether certain parts of the state relation should
+      or should not be enforced.\<close>
+
+record state_rel_options = 
+  consistent_state_rel_opt :: bool
+
 text \<open>The following record abstracts over elements in the Boogie encoding that are used to represent
 Viper counterparts.\<close>
 
@@ -41,6 +47,7 @@ record tr_vpr_bpl =
   fun_translation :: "ViperLang.function_ident \<rightharpoonup> Lang.fname"
   var_translation :: "ViperLang.var \<rightharpoonup> Lang.vname" \<comment>\<open>local Boogie variables\<close>
   const_repr :: "boogie_const \<Rightarrow> Lang.vname"
+  state_rel_opt :: state_rel_options
   
  (*TODO: bound vars*)
 (*  result_var :: "string" *)
@@ -337,40 +344,38 @@ lemma mask_update_wf_apply:
   unfolding mask_update_wf_def
   by blast
 
-definition heap_var_rel :: "ViperLang.program \<Rightarrow>  var_context \<Rightarrow>  'a ty_repr_bpl \<Rightarrow> tr_vpr_bpl \<Rightarrow> vname \<Rightarrow> 'a full_total_state \<Rightarrow> ('a vbpl_absval) nstate \<Rightarrow> bool"
+definition heap_var_rel :: "ViperLang.program \<Rightarrow>  var_context \<Rightarrow>  'a ty_repr_bpl \<Rightarrow> (field_ident \<rightharpoonup> Lang.vname) \<Rightarrow> vname \<Rightarrow> 'a full_total_state \<Rightarrow> ('a vbpl_absval) nstate \<Rightarrow> bool"
   where
-    "heap_var_rel Pr \<Lambda> TyRep T hvar \<omega> ns \<equiv>
+    "heap_var_rel Pr \<Lambda> TyRep FieldTr hvar \<omega> ns \<equiv>
                  (\<exists>hb. lookup_var \<Lambda> ns hvar = Some (AbsV (AHeap hb)) \<and>
                  lookup_var_ty \<Lambda> hvar = Some (TConSingle (THeapId TyRep)) \<and>
                  vbpl_absval_ty_opt TyRep (AHeap hb) = Some ((THeapId TyRep) ,[]) \<and>
-                 heap_rel Pr (field_translation T) (get_hh_total_full \<omega>) hb) \<and>
+                 heap_rel Pr FieldTr (get_hh_total_full \<omega>) hb) \<and>
                  total_heap_well_typed Pr (domain_type TyRep) (get_hh_total_full \<omega>)"
 
-definition mask_var_rel :: "ViperLang.program \<Rightarrow>  var_context \<Rightarrow>  'a ty_repr_bpl \<Rightarrow> tr_vpr_bpl \<Rightarrow> vname \<Rightarrow> 'a full_total_state \<Rightarrow> ('a vbpl_absval) nstate \<Rightarrow> bool"
+definition mask_var_rel :: "ViperLang.program \<Rightarrow>  var_context \<Rightarrow>  'a ty_repr_bpl \<Rightarrow> (field_ident \<rightharpoonup> Lang.vname) \<Rightarrow> vname \<Rightarrow> 'a full_total_state \<Rightarrow> ('a vbpl_absval) nstate \<Rightarrow> bool"
   where
-    "mask_var_rel Pr \<Lambda> TyRep T mvar \<omega> ns \<equiv>
+    "mask_var_rel Pr \<Lambda> TyRep FieldTr mvar \<omega> ns \<equiv>
                  (\<exists>mb. lookup_var \<Lambda> ns mvar = Some (AbsV (AMask mb)) \<and> 
                  lookup_var_ty \<Lambda> mvar = Some (TConSingle (TMaskId TyRep)) \<and> 
              \<comment>\<open>Since all Boogie masks \<^term>\<open>mb\<close> have the correct type, we don't add a typing constraint 
                (in contrast to Boogie heaps).\<close>                 
-                       mask_rel Pr (field_translation T) (get_mh_total_full \<omega>) mb)"
+                       mask_rel Pr FieldTr (get_mh_total_full \<omega>) mb)"
 
 lemma heap_var_rel_stable:
-  assumes "heap_var_rel Pr \<Lambda> TyRep Tr hvar \<omega> ns" and
+  assumes "heap_var_rel Pr \<Lambda> TyRep FieldTr hvar \<omega> ns" and
           "get_hh_total_full \<omega> = get_hh_total_full \<omega>'" and
-          "lookup_var \<Lambda> ns hvar = lookup_var \<Lambda> ns' hvar" and
-          "field_translation Tr = field_translation Tr'"
-        shows "heap_var_rel Pr \<Lambda> TyRep Tr' hvar \<omega>' ns'"
+          "lookup_var \<Lambda> ns hvar = lookup_var \<Lambda> ns' hvar"
+        shows "heap_var_rel Pr \<Lambda> TyRep FieldTr hvar \<omega>' ns'"
   using assms
   unfolding heap_var_rel_def
   by auto
 
 lemma mask_var_rel_stable:
-  assumes "mask_var_rel Pr \<Lambda> TyRep Tr mvar \<omega>' ns"
+  assumes "mask_var_rel Pr \<Lambda> TyRep FieldTr mvar \<omega>' ns"
           "get_mh_total_full \<omega> = get_mh_total_full \<omega>'"
-          "lookup_var \<Lambda> ns mvar = lookup_var \<Lambda> ns' mvar" and
-          "field_translation Tr = field_translation Tr'"
-        shows "mask_var_rel Pr \<Lambda> TyRep Tr' mvar \<omega> ns'"
+          "lookup_var \<Lambda> ns mvar = lookup_var \<Lambda> ns' mvar"
+        shows "mask_var_rel Pr \<Lambda> TyRep FieldTr mvar \<omega> ns'"
   using assms
   unfolding mask_var_rel_def
   by auto
@@ -592,7 +597,6 @@ proof (rule allI | rule impI)+
   qed
 qed
 
-
 definition state_rel0 :: "ViperLang.program \<Rightarrow> 
                           ('a full_total_state \<Rightarrow> bool) \<Rightarrow>
                           ('a vbpl_absval) absval_ty_fun \<Rightarrow> 
@@ -608,9 +612,11 @@ definition state_rel0 :: "ViperLang.program \<Rightarrow>
          \<comment>\<open>field permissions can be at most one\<close>
             wf_mask_simple (get_mh_total_full \<omega>def) \<and>
             wf_mask_simple (get_mh_total_full \<omega>) \<and>
-         \<comment>\<open>the state consistency predicate must hold\<close> 
-            StateCons \<omega>def \<and>
-            StateCons \<omega> \<and>
+         \<comment>\<open>The state consistency predicate must hold if the option is set. The reason for having an
+            option here is because there are cases where one wants to prove the state relation w.r.t.
+            some consistent Viper state via multiple intermediate Viper states that may not be 
+            consistent (in such a case one can temporarily disable the state consistency)\<close> 
+            ((consistent_state_rel_opt (state_rel_opt Tr)) \<longrightarrow> StateCons \<omega>def \<and> StateCons \<omega>) \<and>
          \<comment>\<open>type interpretation must be the expected one\<close>
            (A = vbpl_absval_ty TyRep) \<and>
          \<comment>\<open>Store relation (only Viper variables, auxiliaries are not included)\<close>
@@ -629,11 +635,11 @@ definition state_rel0 :: "ViperLang.program \<Rightarrow>
              get_h_total_full \<omega>def = get_h_total_full \<omega>
            ) \<and>
           \<comment>\<open>heap and mask relation for evaluation state\<close>
-           heap_var_rel Pr \<Lambda> TyRep Tr (heap_var Tr) \<omega> ns \<and>
-           mask_var_rel Pr \<Lambda> TyRep Tr (mask_var Tr) \<omega> ns \<and> 
+           heap_var_rel Pr \<Lambda> TyRep (field_translation Tr) (heap_var Tr) \<omega> ns \<and>
+           mask_var_rel Pr \<Lambda> TyRep (field_translation Tr) (mask_var Tr) \<omega> ns \<and> 
           \<comment>\<open>heap and mask relation for well-definedness state\<close>
-           heap_var_rel Pr \<Lambda> TyRep Tr (heap_var_def Tr) \<omega>def ns \<and>
-           mask_var_rel Pr \<Lambda> TyRep Tr (mask_var_def Tr) \<omega>def ns \<and>      
+           heap_var_rel Pr \<Lambda> TyRep (field_translation Tr) (heap_var_def Tr) \<omega>def ns \<and>
+           mask_var_rel Pr \<Lambda> TyRep (field_translation Tr) (mask_var_def Tr) \<omega>def ns \<and>      
           \<comment>\<open>field relation\<close>
            field_rel Pr \<Lambda> (field_translation Tr) ns \<and>
           \<comment>\<open>Boogie constants relation\<close>
@@ -780,6 +786,7 @@ lemmas state_rel_wf_mask_simple = state_rel0_wf_mask_simple[OF state_rel_state_r
 
 lemma state_rel0_consistent:
   assumes "state_rel0 Pr StateCons A \<Lambda> TyRep Tr AuxPred \<omega>def \<omega> ns"
+      and "consistent_state_rel_opt (state_rel_opt Tr)"
   shows "StateCons \<omega>def \<and> StateCons \<omega>"
   using assms        
   unfolding state_rel0_def
@@ -989,7 +996,7 @@ lemmas state_rel_eval_welldef_eq = state_rel0_eval_welldef_eq[OF state_rel_state
 
 lemma state_rel0_heap_var_rel:
   assumes "state_rel0 Pr StateCons A \<Lambda> TyRep Tr AuxPred \<omega>def \<omega> ns"
-  shows "heap_var_rel Pr \<Lambda> TyRep Tr (heap_var Tr) \<omega> ns"
+  shows "heap_var_rel Pr \<Lambda> TyRep (field_translation Tr) (heap_var Tr) \<omega> ns"
   using assms
   by (simp add: state_rel0_def)
 
@@ -997,7 +1004,7 @@ lemmas state_rel_heap_var_rel = state_rel0_heap_var_rel[OF state_rel_state_rel0]
 
 lemma state_rel0_heap_var_def_rel:
   assumes "state_rel0 Pr StateCons A \<Lambda> TyRep Tr AuxPred \<omega>def \<omega> ns"
-  shows "heap_var_rel Pr \<Lambda> TyRep Tr (heap_var_def Tr) \<omega>def ns"
+  shows "heap_var_rel Pr \<Lambda> TyRep (field_translation Tr) (heap_var_def Tr) \<omega>def ns"
   using assms
   by (simp add: state_rel0_def)
 
@@ -1005,7 +1012,7 @@ lemmas state_rel_heap_var_def_rel = state_rel0_heap_var_def_rel[OF state_rel_sta
 
 lemma state_rel0_mask_var_rel:
   assumes "state_rel0 Pr StateCons A \<Lambda> TyRep Tr AuxPred \<omega>def \<omega> ns"
-  shows "mask_var_rel Pr \<Lambda> TyRep Tr (mask_var Tr) \<omega> ns"
+  shows "mask_var_rel Pr \<Lambda> TyRep (field_translation Tr) (mask_var Tr) \<omega> ns"
   using assms
   by (simp add: state_rel0_def)
 
@@ -1013,7 +1020,7 @@ lemmas state_rel_mask_var_rel = state_rel0_mask_var_rel[OF state_rel_state_rel0]
 
 lemma state_rel0_mask_var_def_rel:
   assumes "state_rel0 Pr StateCons A \<Lambda> TyRep Tr AuxPred \<omega>def \<omega> ns"
-  shows "mask_var_rel Pr \<Lambda> TyRep Tr (mask_var_def Tr) \<omega>def ns"
+  shows "mask_var_rel Pr \<Lambda> TyRep (field_translation Tr) (mask_var_def Tr) \<omega>def ns"
   using assms
   by (simp add: state_rel0_def)
 
@@ -1312,7 +1319,7 @@ lemma state_rel0_store_update:
   assumes StateRel: "state_rel0 Pr StateCons A \<Lambda> TyRep Tr AuxPred \<omega>def \<omega> ns" and
                     "Tr' = Tr\<lparr>var_translation := f\<rparr>" and
           WellDefSame: "\<omega>def = \<omega> \<and> \<omega>def' = \<omega>'" and
-        Consistent: "StateCons \<omega>'" and
+        Consistent: "consistent_state_rel_opt (state_rel_opt Tr') \<Longrightarrow> StateCons \<omega>'" and
      OnlyStoreAffectedVpr: 
            "get_total_full \<omega> = get_total_full \<omega>'"  and
          (*  "get_m_total_full \<omega> = get_m_total_full \<omega>'" and*) 
@@ -1358,7 +1365,7 @@ proof (intro conjI)
       by (simp add: \<open>Tr' = _\<close>)
   qed
 
-  show "heap_var_rel Pr \<Lambda> TyRep Tr' (heap_var Tr') \<omega>' ns'"
+  show "heap_var_rel Pr \<Lambda> TyRep (field_translation Tr') (heap_var Tr') \<omega>' ns'"
   proof -
     have "lookup_var \<Lambda> ns (heap_var Tr) = lookup_var \<Lambda> ns' (heap_var Tr)"
     proof -
@@ -1374,7 +1381,7 @@ proof (intro conjI)
     by (auto simp: \<open>Tr' = _\<close>)
   qed
 
-  show "heap_var_rel Pr \<Lambda> TyRep Tr' (heap_var_def Tr') \<omega>def' ns'"
+  show "heap_var_rel Pr \<Lambda> TyRep (field_translation Tr') (heap_var_def Tr') \<omega>def' ns'"
   proof -   
     have "lookup_var \<Lambda> ns (heap_var_def Tr) = lookup_var \<Lambda> ns' (heap_var_def Tr)"
     proof -
@@ -1391,7 +1398,7 @@ proof (intro conjI)
     by (simp add: \<open>Tr' = _\<close>)
   qed
 
-  show "mask_var_rel Pr \<Lambda> TyRep Tr' (mask_var Tr') \<omega>' ns'"
+  show "mask_var_rel Pr \<Lambda> TyRep (field_translation Tr') (mask_var Tr') \<omega>' ns'"
   proof -  
     have "lookup_var \<Lambda> ns (mask_var Tr) = lookup_var \<Lambda> ns' (mask_var Tr)"
     proof -
@@ -1407,7 +1414,7 @@ proof (intro conjI)
     by (auto simp: \<open>Tr' = _\<close>)
   qed 
 
-  show "mask_var_rel Pr \<Lambda> TyRep Tr' (mask_var_def Tr') \<omega>def' ns'"
+  show "mask_var_rel Pr \<Lambda> TyRep (field_translation Tr') (mask_var_def Tr') \<omega>def' ns'"
   proof -  
     have "lookup_var \<Lambda> ns (mask_var_def Tr) = lookup_var \<Lambda> ns' (mask_var_def Tr)"
     proof -
@@ -1582,19 +1589,19 @@ proof -
       using AuxVarFresh disjoint_list_add[OF *]
       by auto
   next
-    show "heap_var_rel Pr (var_context ctxt) TyRep Tr (heap_var Tr) \<omega> (update_var (var_context ctxt) ns aux_var aux_val)"
+    show "heap_var_rel Pr (var_context ctxt) TyRep (field_translation Tr) (heap_var Tr) \<omega> (update_var (var_context ctxt) ns aux_var aux_val)"
       using heap_var_rel_stable[OF state_rel0_heap_var_rel[OF StateRel0]] AuxVarFresh
       by simp
   next
-    show "mask_var_rel Pr (var_context ctxt) TyRep Tr (mask_var Tr) \<omega> (update_var (var_context ctxt) ns aux_var aux_val)"
+    show "mask_var_rel Pr (var_context ctxt) TyRep (field_translation Tr) (mask_var Tr) \<omega> (update_var (var_context ctxt) ns aux_var aux_val)"
       using mask_var_rel_stable[OF state_rel0_mask_var_rel[OF StateRel0]] AuxVarFresh
       by auto
   next
-    show "heap_var_rel Pr (var_context ctxt) TyRep Tr (heap_var_def Tr) \<omega>def (update_var (var_context ctxt) ns aux_var aux_val)"
+    show "heap_var_rel Pr (var_context ctxt) TyRep (field_translation Tr) (heap_var_def Tr) \<omega>def (update_var (var_context ctxt) ns aux_var aux_val)"
       using heap_var_rel_stable[OF state_rel0_heap_var_def_rel[OF StateRel0]] AuxVarFresh
       by simp
   next
-    show "mask_var_rel Pr (var_context ctxt) TyRep Tr (mask_var_def Tr) \<omega>def (update_var (var_context ctxt) ns aux_var aux_val)"
+    show "mask_var_rel Pr (var_context ctxt) TyRep (field_translation Tr) (mask_var_def Tr) \<omega>def (update_var (var_context ctxt) ns aux_var aux_val)"
       using mask_var_rel_stable[OF state_rel0_mask_var_def_rel[OF StateRel0]] AuxVarFresh
       by auto
   next
@@ -1688,10 +1695,10 @@ lemma state_rel0_heap_update:
                       dom AuxPred) = {}" and
           UpdStates: "\<omega>def' = update_h_total_full \<omega>def hh' hp'" 
                      "\<omega>' = update_h_total_full \<omega> hh' hp'" and
-          Consistent: "StateCons \<omega>def'" "StateCons \<omega>'" and
+          Consistent: "consistent_state_rel_opt (state_rel_opt Tr) \<Longrightarrow> StateCons \<omega>def' \<and> StateCons \<omega>'" and
           OnlyHeapAffected: "(\<And>x. x \<notin> {hvar', hvar_def'} \<Longrightarrow> lookup_var \<Lambda> ns x = lookup_var \<Lambda> ns' x)" and
-          HeapRel: "heap_var_rel Pr \<Lambda> TyRep Tr hvar' \<omega>' ns'" and
-          HeapRelDef: "heap_var_rel Pr \<Lambda> TyRep Tr hvar_def' \<omega>def' ns'" and
+          HeapRel: "heap_var_rel Pr \<Lambda> TyRep (field_translation Tr) hvar' \<omega>' ns'" and
+          HeapRelDef: "heap_var_rel Pr \<Lambda> TyRep (field_translation Tr) hvar_def' \<omega>def' ns'" and
           ShadowedGlobalsEq: "\<And>x. map_of (snd \<Lambda>) x \<noteq> None \<Longrightarrow> global_state ns' x = global_state ns x" and
           OldStateEq: "old_global_state ns' = old_global_state ns" and
           BinderEmpty: "binder_state ns' = Map.empty"
@@ -1719,24 +1726,22 @@ lemma state_rel0_heap_update:
         by blast      
     qed
   next  
-    have "mask_var_rel Pr \<Lambda> TyRep Tr' (mask_var Tr) \<omega>' ns'"      
+    have "mask_var_rel Pr \<Lambda> TyRep (field_translation Tr) (mask_var Tr) \<omega>' ns'"      
       apply (rule mask_var_rel_stable[OF state_rel0_mask_var_rel[OF StateRel]])
       using \<open>\<omega>' = _\<close>
        apply simp
       using OnlyHeapAffected Disj
-      apply force      
-      by (simp add: \<open>Tr' = _\<close>)
-    thus "mask_var_rel Pr \<Lambda> TyRep Tr' (mask_var Tr') \<omega>' ns'"
+      by force      
+    thus "mask_var_rel Pr \<Lambda> TyRep (field_translation Tr') (mask_var Tr') \<omega>' ns'"
       by (simp add: \<open>Tr' = _\<close>)
   next
-    have "mask_var_rel Pr \<Lambda> TyRep Tr' (mask_var_def Tr) \<omega>def' ns'"
+    have "mask_var_rel Pr \<Lambda> TyRep (field_translation Tr) (mask_var_def Tr) \<omega>def' ns'"
           apply (rule mask_var_rel_stable[OF state_rel0_mask_var_def_rel[OF StateRel]])
       using \<open>\<omega>def' = _\<close>
        apply simp
       using mask_var_disjoint[OF StateRel] OnlyHeapAffected Disj
-       apply force
-      by (simp add: \<open>Tr' = _\<close>)
-    thus "mask_var_rel Pr \<Lambda> TyRep Tr' (mask_var_def Tr') \<omega>def' ns'"
+      by force
+    thus "mask_var_rel Pr \<Lambda> TyRep (field_translation Tr') (mask_var_def Tr') \<omega>def' ns'"
       by (simp add: \<open>Tr' = _\<close>)
   next
     show "field_rel Pr \<Lambda> (field_translation Tr') ns'"
@@ -1816,12 +1821,12 @@ next
     apply (rule disjoint_list_subset_list_all2)
     by (simp add: \<open>Tr' = _\<close>)
 next
-  show "heap_var_rel Pr \<Lambda> TyRep Tr' (heap_var Tr') \<omega>' ns'"
+  show "heap_var_rel Pr \<Lambda> TyRep (field_translation Tr') (heap_var Tr') \<omega>' ns'"
     using HeapRel \<open>Tr' = _\<close> 
     unfolding heap_var_rel_def
     by auto    
 next
-  show "heap_var_rel Pr \<Lambda> TyRep Tr' (heap_var_def Tr') \<omega>def' ns'"
+  show "heap_var_rel Pr \<Lambda> TyRep (field_translation Tr') (heap_var_def Tr') \<omega>def' ns'"
     using HeapRelDef \<open>Tr' = _\<close> 
     unfolding heap_var_rel_def
     by auto
@@ -1832,18 +1837,18 @@ lemmas state_rel_heap_update =
 
 lemma state_rel0_heap_update_2:
   assumes                                
-     StateRel: "state_rel0 Pr StateCons TyInterp \<Lambda> TyRep Tr AuxPred \<omega>def \<omega> ns" and
-          TyInterp:     "TyInterp = vbpl_absval_ty TyRep" and
-          WellDefSame: "\<omega>def = \<omega> \<and> \<omega>def' = \<omega>' \<and> heap_var Tr = heap_var_def Tr" and
-          Consistent: "StateCons \<omega>'" and
-          OnlyHeapAffected: "(\<And>x. x \<noteq> heap_var Tr \<Longrightarrow> lookup_var \<Lambda> ns x = lookup_var \<Lambda> ns' x)" and
-          OnlyHeapAffectedVpr: "get_store_total \<omega> = get_store_total \<omega>'" 
-                               "get_m_total_full \<omega> = get_m_total_full \<omega>'"
-                               "get_trace_total \<omega> = get_trace_total \<omega>'" and
-          HeapRel: "heap_var_rel Pr \<Lambda> TyRep Tr (heap_var Tr) \<omega>' ns'" and
-          ShadowedGlobalsEq: "\<And>x. map_of (snd \<Lambda>) x \<noteq> None \<Longrightarrow> global_state ns' x = global_state ns x" and
-          OldStateEq: "old_global_state ns' = old_global_state ns" and
-          BinderEmpty: "binder_state ns' = Map.empty"
+    StateRel: "state_rel0 Pr StateCons TyInterp \<Lambda> TyRep Tr AuxPred \<omega>def \<omega> ns" and
+    TyInterp:     "TyInterp = vbpl_absval_ty TyRep" and
+    WellDefSame: "\<omega>def = \<omega> \<and> \<omega>def' = \<omega>' \<and> heap_var Tr = heap_var_def Tr" and
+    Consistent: "consistent_state_rel_opt (state_rel_opt Tr) \<Longrightarrow> StateCons \<omega>'" and
+    OnlyHeapAffected: "(\<And>x. x \<noteq> heap_var Tr \<Longrightarrow> lookup_var \<Lambda> ns x = lookup_var \<Lambda> ns' x)" and
+    OnlyHeapAffectedVpr: "get_store_total \<omega> = get_store_total \<omega>'" 
+                         "get_m_total_full \<omega> = get_m_total_full \<omega>'"
+                         "get_trace_total \<omega> = get_trace_total \<omega>'" and
+    HeapRel: "heap_var_rel Pr \<Lambda> TyRep (field_translation Tr) (heap_var Tr) \<omega>' ns'" and
+    ShadowedGlobalsEq: "\<And>x. map_of (snd \<Lambda>) x \<noteq> None \<Longrightarrow> global_state ns' x = global_state ns x" and
+    OldStateEq: "old_global_state ns' = old_global_state ns" and
+    BinderEmpty: "binder_state ns' = Map.empty"
         shows "state_rel0 Pr StateCons TyInterp \<Lambda> TyRep Tr AuxPred \<omega>def' \<omega>' ns'"  
 proof (rule state_rel0_heap_update[OF StateRel TyInterp])
   show "Tr = Tr\<lparr>heap_var := heap_var Tr, heap_var_def := heap_var_def Tr\<rparr>"
@@ -1877,16 +1882,16 @@ lemmas state_rel_heap_update_2 =
 lemma heap_var_rel_update:
   assumes 
      WfTyRep: "wf_ty_repr_bpl TyRep" and
-     HeapVarRel: "heap_var_rel Pr \<Lambda> TyRep Tr (heap_var Tr) \<omega> ns" and
+     HeapVarRel: "heap_var_rel Pr \<Lambda> TyRep (field_translation Tr) (heap_var Tr) \<omega> ns" and
      LookupHeapVar: "lookup_var \<Lambda> ns (heap_var Tr) = Some (AbsV (AHeap hb))" and
      FieldLookup: "declared_fields Pr f_vpr = Some ty_vpr" and
                "vpr_to_bpl_ty TyRep ty_vpr = Some ty_bpl" and
      VVprTy:   "get_type (domain_type TyRep) v_vpr = ty_vpr" and
      FieldTranslation: "field_translation Tr f_vpr = Some f_bpl" and
      FieldTranslationInj: "inj_on (field_translation Tr) (dom (field_translation Tr))"
-  shows "heap_var_rel Pr \<Lambda> TyRep Tr (heap_var Tr) (update_hh_loc_total_full \<omega> (addr, f_vpr) v_vpr)
+  shows "heap_var_rel Pr \<Lambda> TyRep (field_translation Tr) (heap_var Tr) (update_hh_loc_total_full \<omega> (addr, f_vpr) v_vpr)
      (update_var \<Lambda> ns (heap_var Tr) (AbsV (AHeap (heap_bpl_upd_normal_field hb (Address addr) f_bpl ty_vpr (val_rel_vpr_bpl v_vpr)))))"
-      (is "heap_var_rel Pr \<Lambda> TyRep Tr (heap_var Tr) ?\<omega>' ?ns'")
+      (is "heap_var_rel Pr \<Lambda> TyRep _ (heap_var Tr) ?\<omega>' ?ns'")
 proof -
   from HeapVarRel and LookupHeapVar have
    HeapRelFacts:
@@ -1950,7 +1955,6 @@ proof -
       qed
     qed
   next
-    thm vpr_to_bpl_val_type
     show "total_heap_well_typed Pr (domain_type TyRep)(get_hh_total_full (update_hh_loc_total_full \<omega> (addr, f_vpr) v_vpr))"
       unfolding total_heap_well_typed_def
     proof (rule allI | rule impI)+
@@ -1979,8 +1983,7 @@ lemma state_rel_heap_update_3:
      WfTyRep: "wf_ty_repr_bpl TyRep" and
      StateRel: "state_rel Pr StateCons TyRep Tr AuxPred ctxt \<omega>def \<omega> ns" and
      WellDefSame: "\<omega>def = \<omega> \<and> heap_var Tr = heap_var_def Tr" and
-     Consistent: "StateCons (update_hh_loc_total_full \<omega>def (addr, f_vpr) v_vpr)" 
-                 "StateCons (update_hh_loc_total_full \<omega> (addr, f_vpr) v_vpr)" and
+     Consistent: "consistent_state_rel_opt (state_rel_opt Tr) \<Longrightarrow> StateCons (update_hh_loc_total_full \<omega>def (addr, f_vpr) v_vpr) \<and> StateCons (update_hh_loc_total_full \<omega> (addr, f_vpr) v_vpr)" and
      LookupHeap:  "lookup_var (var_context ctxt) ns (heap_var Tr) = Some (AbsV (AHeap hb))" and
      FieldLookup: "declared_fields Pr f_vpr = Some ty_vpr" and
      FieldTranslation: "field_translation Tr f_vpr = Some f_bpl" and
@@ -2001,7 +2004,7 @@ next
   show "get_m_total_full \<omega> = get_m_total_full ?\<omega>'"
     by simp
 next
-  show "heap_var_rel Pr (var_context ctxt) TyRep Tr (heap_var Tr) ?\<omega>' ?ns'"
+  show "heap_var_rel Pr (var_context ctxt) TyRep (field_translation Tr) (heap_var Tr) ?\<omega>' ?ns'"
     apply (rule heap_var_rel_update[OF WfTyRep])
     using state_rel_state_rel0[OF StateRel] assms
     unfolding state_rel0_def field_rel_def
@@ -2026,8 +2029,8 @@ lemma state_rel_heap_update_2_ext:
      WfTyRep: "wf_ty_repr_bpl TyRep" and
      StateRel: "state_rel Pr StateCons TyRep Tr AuxPred ctxt \<omega>def \<omega> ns" and
      WellDefSame: "\<omega>def = \<omega> \<and> heap_var Tr = heap_var_def Tr" and
-     Consistent: "StateCons (update_hh_loc_total_full \<omega>def (addr, f_vpr) v)" 
-                 "StateCons (update_hh_loc_total_full \<omega> (addr, f_vpr) v)" and
+     Consistent: "consistent_state_rel_opt (state_rel_opt Tr) \<Longrightarrow> StateCons (update_hh_loc_total_full \<omega>def (addr, f_vpr) v)"
+                 "consistent_state_rel_opt (state_rel_opt Tr) \<Longrightarrow> StateCons (update_hh_loc_total_full \<omega> (addr, f_vpr) v)" and
      FieldLookup: "declared_fields Pr f_vpr = Some ty_vpr" and
      FieldTranslation: "field_translation Tr f_vpr = Some f_bpl" and
      TyTranslation: "vpr_to_bpl_ty TyRep ty_vpr = Some ty_bpl" and
@@ -2091,10 +2094,9 @@ lemma state_rel0_mask_update:
           OnlyMaskAffected: "\<And>x. x \<notin> {mvar', mvar_def'} \<Longrightarrow> lookup_var \<Lambda> ns x = lookup_var \<Lambda> ns' x" and
           WfMaskSimple: "wf_mask_simple mh'" 
                         "wf_mask_simple (get_mh_total_full \<omega>def')" and
-          Consistent: "StateCons \<omega>'" 
-                      "StateCons \<omega>def'" and
-          MaskVarRel: "mask_var_rel Pr \<Lambda> TyRep Tr mvar' \<omega>' ns'" 
-                      "mask_var_rel Pr \<Lambda> TyRep Tr mvar_def' \<omega>def' ns'" and
+          Consistent: "consistent_state_rel_opt (state_rel_opt Tr) \<Longrightarrow> StateCons \<omega>' \<and> StateCons \<omega>def'" and 
+          MaskVarRel: "mask_var_rel Pr \<Lambda> TyRep (field_translation Tr) mvar' \<omega>' ns'" 
+                      "mask_var_rel Pr \<Lambda> TyRep (field_translation Tr) mvar_def' \<omega>def' ns'" and
           ShadowedGlobalsEq: "\<And>x. map_of (snd \<Lambda>) x \<noteq> None \<Longrightarrow> global_state ns' x = global_state ns x" and
           OldStateEq: "old_global_state ns' = old_global_state ns" and
           BinderEmpty: "binder_state ns' = Map.empty"
@@ -2114,20 +2116,19 @@ proof (intro conjI)
       by blast      
   qed
 next
-  show "heap_var_rel Pr \<Lambda> TyRep Tr' (heap_var Tr') \<omega>' ns'"
+  show "heap_var_rel Pr \<Lambda> TyRep (field_translation Tr') (heap_var Tr') \<omega>' ns'"
     using Disj OnlyMaskAffected
     by (fastforce intro!: heap_var_rel_stable[OF state_rel0_heap_var_rel[OF StateRel]]
                        simp: \<open>Tr' = _\<close> \<open>\<omega>' = _\<close>)
 next
-  have HeapVarRelDef: "heap_var_rel Pr \<Lambda> TyRep Tr' (heap_var_def Tr) \<omega>def' ns'"
+  have HeapVarRelDef: "heap_var_rel Pr \<Lambda> TyRep (field_translation Tr) (heap_var_def Tr) \<omega>def' ns'"
     apply (rule heap_var_rel_stable[OF state_rel0_heap_var_def_rel[OF StateRel]])
     using UpdStates StateRel
     unfolding state_rel0_def
       apply simp
     using Disj OnlyMaskAffected
-     apply blast
-    by (simp add: \<open>Tr' = _\<close>)
-  thus "heap_var_rel Pr \<Lambda> TyRep Tr' (heap_var_def Tr') \<omega>def' ns'"
+    by blast
+  thus "heap_var_rel Pr \<Lambda> TyRep (field_translation Tr') (heap_var_def Tr') \<omega>def' ns'"
     by (simp add: \<open>Tr' = _\<close>)
 next
   show "field_rel Pr \<Lambda> (field_translation Tr') ns'"
@@ -2218,8 +2219,8 @@ lemma state_rel0_mask_update_2:
                                "get_trace_total \<omega> = get_trace_total \<omega>'"
                                "get_h_total_full \<omega> = get_h_total_full \<omega>'" and
           WfMaskSimple: "wf_mask_simple (get_mh_total_full \<omega>')" and
-          Consistent: "StateCons \<omega>'" and
-          MaskVarRel: "mask_var_rel Pr \<Lambda> TyRep Tr (mask_var Tr) \<omega>' ns'" and
+          Consistent: "consistent_state_rel_opt (state_rel_opt Tr) \<Longrightarrow> StateCons \<omega>'" and
+          MaskVarRel: "mask_var_rel Pr \<Lambda> TyRep (field_translation Tr) (mask_var Tr) \<omega>' ns'" and
           ShadowedGlobalsEq: "\<And>x. map_of (snd \<Lambda>) x \<noteq> None \<Longrightarrow> global_state ns' x = global_state ns x" and
           OldStateEq: "old_global_state ns' = old_global_state ns" and
           BinderEmpty: "binder_state ns' = Map.empty"
@@ -2237,7 +2238,7 @@ proof -
       using WellDefSame \<open>\<omega>' = _\<close>
       by presburger
 
-    have MaskVarRelDef: "mask_var_rel Pr \<Lambda> TyRep Tr (mask_var_def Tr) \<omega>def' ns'"
+    have MaskVarRelDef: "mask_var_rel Pr \<Lambda> TyRep (field_translation Tr) (mask_var_def Tr) \<omega>def' ns'"
       using MaskVarRel \<open>\<omega>def' = _\<close> True
       unfolding mask_var_rel_def 
       by simp
@@ -2255,7 +2256,6 @@ proof -
             apply simp
       using WfMaskSimple  \<open>\<omega>def' = _\<close>
              apply simp
-            apply (rule Consistent)
       using Consistent state_rel0_consistent[OF StateRel] WellDefSame
            apply blast      
           apply (rule MaskVarRel)
@@ -2274,7 +2274,7 @@ proof -
       unfolding state_rel0_def
       by presburger 
      
-    have MaskVarRelDef: "mask_var_rel Pr \<Lambda> TyRep Tr (mask_var_def Tr) \<omega>def' ns'"
+    have MaskVarRelDef: "mask_var_rel Pr \<Lambda> TyRep (field_translation Tr) (mask_var_def Tr) \<omega>def' ns'"
       using state_rel0_mask_var_def_rel[OF StateRel]
       by (metis False OnlyMaskAffected \<open>\<omega>def' = \<omega>def\<close> mask_var_rel_stable)
       
@@ -2289,7 +2289,6 @@ proof -
             apply (rule WfMaskSimple)
       using \<open>\<omega>def' = _\<close> state_rel0_wf_mask_def_simple[OF StateRel]
              apply blast
-            apply (rule Consistent)
       using Consistent state_rel0_consistent[OF StateRel] WellDefSame
            apply blast
           apply (rule MaskVarRel)
@@ -2305,7 +2304,7 @@ lemma state_rel_mask_update_2b:
   assumes StateRel: "state_rel Pr StateCons TyRep Tr AuxPred ctxt \<omega>def \<omega> ns" and
           WellDefSame: "mask_var Tr = mask_var_def Tr \<and> \<omega>def = \<omega>" and
           OnlyMaskAffected: "\<And>x. x \<noteq> mask_var Tr \<Longrightarrow> lookup_var (var_context ctxt) ns x = lookup_var (var_context ctxt) ns' x" and
-          MaskRel: "mask_var_rel Pr (var_context ctxt) TyRep Tr (mask_var Tr) \<omega> ns'" and
+          MaskRel: "mask_var_rel Pr (var_context ctxt) TyRep (field_translation Tr) (mask_var Tr) \<omega> ns'" and
           ShadowedGlobalsEq: "\<And>x. map_of (snd (var_context ctxt)) x \<noteq> None \<Longrightarrow> global_state ns' x = global_state ns x" and
           OldStateEq: "old_global_state ns' = old_global_state ns" and
           BinderEmpty: "binder_state ns' = Map.empty" and
@@ -2331,21 +2330,21 @@ lemma state_rel_mask_update_3:
   apply (rule exI[where ?x=m'])
   using MaskRel Eq
   apply (meson StateRel state_rel_obtain_mask update_var_same)
-      apply (simp add: Eq)
-      using StateRel
-         apply (metis assms(4) global_state_update_local global_state_update_other)
-        apply (simp add: update_var_old_global_same)
-      using state_rel0_state_well_typed[OF state_rel_state_rel0[OF StateRel]]
-      unfolding state_well_typed_def
-      apply (simp add: update_var_binder_same)
-      by (simp add: TypeInterp)
+  apply (simp add: Eq)
+  using StateRel
+     apply (metis assms(4) global_state_update_local global_state_update_other)
+    apply (simp add: update_var_old_global_same)
+  using state_rel0_state_well_typed[OF state_rel_state_rel0[OF StateRel]]
+  unfolding state_well_typed_def
+  apply (simp add: update_var_binder_same)
+  by (simp add: TypeInterp)
 
 lemma state_rel_mask_update_4:
   assumes StateRel: "state_rel Pr StateCons TyRep Tr AuxPred ctxt \<omega>def \<omega> ns" and 
                     "\<Lambda> = (var_context ctxt)" and
           WellDefSame: "mask_var Tr = mask_var_def Tr \<Longrightarrow> \<omega>def' = update_mh_loc_total_full \<omega> (addr, f_vpr) p"
                        "mask_var Tr \<noteq> mask_var_def Tr \<Longrightarrow> \<omega>def' = \<omega>def"  and
-        Consistent: "StateCons (update_mh_loc_total_full \<omega> (addr, f_vpr) p)" and
+        Consistent: "consistent_state_rel_opt (state_rel_opt Tr) \<Longrightarrow> StateCons (update_mh_loc_total_full \<omega> (addr, f_vpr) p)" and
         TypeInterp: "type_interp ctxt = vbpl_absval_ty TyRep" and
         LookupMask: "lookup_var (var_context ctxt) ns (mask_var Tr) = Some (AbsV (AMask mb))" and
                     "pgte pwrite p" and
@@ -2454,7 +2453,7 @@ next
       by auto
   qed
 
-  thus "mask_var_rel Pr (var_context ctxt) TyRep Tr (mask_var Tr) ?\<omega>' ?ns'"
+  thus "mask_var_rel Pr (var_context ctxt) TyRep (field_translation Tr) (mask_var Tr) ?\<omega>' ?ns'"
     using state_rel0_mask_var_rel[OF state_rel_state_rel0[OF StateRel]]
     unfolding mask_var_rel_def
     using \<open>\<Lambda> = _\<close> update_var_same \<open>p_bpl = _\<close> by blast
@@ -2495,7 +2494,7 @@ qed (insert StateRel,
 
 lemma state_rel_mask_var_def_update:
   assumes StateRel: "state_rel Pr StateCons TyRep Tr AuxPred ctxt \<omega>def \<omega> ns" and  
-   MaskVarRel: "mask_var_rel Pr (var_context ctxt) TyRep (Tr\<lparr>mask_var_def := mvar_def'\<rparr>) mvar_def' \<omega>def ns" and
+   MaskVarRel: "mask_var_rel Pr (var_context ctxt) TyRep (field_translation Tr) mvar_def' \<omega>def ns" and
           VarFresh: "mvar_def' \<notin> ({heap_var Tr, heap_var_def Tr, mask_var Tr} \<union>
                       (ran (var_translation Tr)) \<union>
                       (ran (field_translation Tr)) \<union>
@@ -2534,7 +2533,7 @@ proof (intro conjI)
       ran (field_translation (Tr\<lparr>mask_var_def := mvar_def'\<rparr>)), range (const_repr (Tr\<lparr>mask_var_def := mvar_def'\<rparr>)), dom AuxPred]"
       by auto
 next
-  show "mask_var_rel Pr (var_context ctxt) TyRep (Tr\<lparr>mask_var_def := mvar_def'\<rparr>) (mask_var_def (Tr\<lparr>mask_var_def := mvar_def'\<rparr>)) \<omega>def ns"
+  show "mask_var_rel Pr (var_context ctxt) TyRep (field_translation (Tr\<lparr>mask_var_def := mvar_def'\<rparr>)) (mask_var_def (Tr\<lparr>mask_var_def := mvar_def'\<rparr>)) \<omega>def ns"
     using MaskVarRel
     by simp
 qed (insert StateRel,
@@ -2550,7 +2549,7 @@ qed (insert StateRel,
 
 lemma state_rel_heap_var_def_update:
   assumes StateRel: "state_rel Pr StateCons TyRep Tr AuxPred ctxt \<omega>def \<omega> ns" and
-          HeapVarRel: "heap_var_rel Pr (var_context ctxt) TyRep (Tr\<lparr>heap_var_def := hvar_def'\<rparr>) hvar_def' \<omega>def ns" and
+          HeapVarRel: "heap_var_rel Pr (var_context ctxt) TyRep (field_translation Tr) hvar_def' \<omega>def ns" and
           VarFresh: "hvar_def' \<notin> ({heap_var Tr, mask_var Tr, mask_var_def Tr} \<union>
                       (ran (var_translation Tr)) \<union>
                       (ran (field_translation Tr)) \<union>
@@ -2590,7 +2589,7 @@ proof (intro conjI)
       ran (field_translation (Tr\<lparr>heap_var_def := hvar_def'\<rparr>)), range (const_repr (Tr\<lparr>heap_var_def := hvar_def'\<rparr>)), dom AuxPred]"
       by auto
 next
-  show "heap_var_rel Pr (var_context ctxt) TyRep (Tr\<lparr>heap_var_def := hvar_def'\<rparr>) (heap_var_def (Tr\<lparr>heap_var_def := hvar_def'\<rparr>)) \<omega>def ns"
+  show "heap_var_rel Pr (var_context ctxt) TyRep (field_translation (Tr\<lparr>heap_var_def := hvar_def'\<rparr>)) (heap_var_def (Tr\<lparr>heap_var_def := hvar_def'\<rparr>)) \<omega>def ns"
     using HeapVarRel
     by fastforce
 qed (insert StateRel,
@@ -2603,6 +2602,36 @@ qed (insert StateRel,
      insert field_rel_stable[OF state_rel_field_rel[OF StateRel]],
      insert boogie_const_rel_stable[OF state_rel_boogie_const_rel[OF StateRel]],
      auto)
+
+subsection \<open>Adjust state relation options\<close>
+
+abbreviation disable_consistent_state_rel_opt :: "tr_vpr_bpl \<Rightarrow> tr_vpr_bpl"
+  where "disable_consistent_state_rel_opt Tr \<equiv> Tr \<lparr> state_rel_opt := (state_rel_opt Tr) \<lparr> consistent_state_rel_opt := False \<rparr> \<rparr>"
+
+abbreviation enable_consistent_state_rel_opt :: "tr_vpr_bpl \<Rightarrow> tr_vpr_bpl"
+  where "enable_consistent_state_rel_opt Tr \<equiv> Tr \<lparr> state_rel_opt := (state_rel_opt Tr) \<lparr> consistent_state_rel_opt := True \<rparr> \<rparr>"
+
+lemma state_rel_disable_consistency:
+  assumes  "state_rel Pr StateCons TyRep Tr AuxPred ctxt \<omega>def \<omega> ns"       
+  shows "state_rel Pr StateCons TyRep (disable_consistent_state_rel_opt Tr) AuxPred ctxt \<omega>def \<omega> ns"
+  unfolding state_rel_def state_rel0_def
+  by (insert assms[simplified state_rel_def state_rel0_def]) auto
+
+lemma state_rel_enable_consistency:
+  assumes "state_rel Pr StateCons TyRep Tr AuxPred ctxt \<omega>def \<omega> ns" 
+      and "StateCons \<omega> \<and> StateCons \<omega>def"       
+    shows "state_rel Pr StateCons TyRep (enable_consistent_state_rel_opt Tr) AuxPred ctxt \<omega>def \<omega> ns"
+  unfolding state_rel_def state_rel0_def
+  by (insert assms[simplified state_rel_def state_rel0_def]) auto
+
+lemma state_rel_enable_consistency_2:
+  assumes "state_rel Pr StateCons TyRep Tr' AuxPred ctxt \<omega>def \<omega> ns" 
+      and "Tr' = (disable_consistent_state_rel_opt Tr)"
+      and "StateCons \<omega> \<and> StateCons \<omega>def"       
+    shows "state_rel Pr StateCons TyRep Tr AuxPred ctxt \<omega>def \<omega> ns"
+  unfolding state_rel_def state_rel0_def
+  by (insert assms[simplified state_rel_def state_rel0_def]) auto
+  
 
 subsection\<open>function relation\<close>
 
